\newpage
\section{Additional Heap Functions}
\label{sec:heap-additional}
\begin{lstlisting}[caption={Merging heaps},label={lst:appendix:heap:merge}]
tListMergeAm\equiv :  {l acc acc' : bNat}
              -> (left : SparseTreeList A l acc)
              -> (right : SparseTreeList A l acc')
              -> Am1 (tlist-amortized' A) A l
tListMergeAm\equiv {l = l} {acc' = acc'} [] right =
                Am1.step {nextA = const l} {nextI = const acc'} {time = const 0}
                (lift1 0) (\lambda _ -> return right)
tListMergeAm\equiv {l = l} {acc = acc} (empty:: left) [] =
                Am1.step {nextA = const l} {nextI = const acc} {time = const 0}
                (lift1 0) (\lambda _ -> return $ empty:: left)
tListMergeAm\equiv (empty:: left) (empty:: right) =
                Am1.step {nextA = pred} {nextI = ts-acc} {time = const 0}
                (tListMergeAm\equiv left right) (\lambda ts -> return $ empty:: ts)
tListMergeAm\equiv {l = l} (empty:: left) (entry x :: right) =
                Am1.step {nextA = pred} {nextI = \lambda ts -> 2 ^ l + ts-acc ts} {time = const 0}
                (tListMergeAm\equiv left right) (\lambda ts -> return $ entry_::_ {acc' = 2 ^ l + ts-acc ts} {acc'\equiv2^l+acc = refl} x ts)
tListMergeAm\equiv {l = l} {acc = acc} left@(entry _ :: _) [] =
                Am1.step {nextA = const l} {nextI = const acc} {time = const 0}
                (lift1 0) (\lambda _ -> return left)
tListMergeAm\equiv {l = l} (entry x :: left) (empty:: right) =
                Am1.step {nextA = pred} {nextI = \lambda ts -> 2 ^ l + ts-acc ts } {time = const 0}
                (tListMergeAm\equiv left right) (\lambda ts -> return $ entry_::_ {acc' = 2 ^ l + ts-acc ts} {acc'\equiv2^l+acc = refl} x ts)
tListMergeAm\equiv {l = l} (entry x :: left) (entry y :: right) =
                Am1.step {nextA = pred} {nextI = \lambda ts -> 2 ^ (suc l) + ts-acc ts} {time = \lambda ts -> suc $ leadingEntries ts}
                (tListMergeAm\equiv left right)
                (\lambda ts -> link x y >>= \lambda t-join -> empty:: <$> insertTList\equiv t-join ts)

tListMergeAm\leq :  {l l' acc acc' : bNat}
              -> l \leq l'
              -> (left : SparseTreeList A l acc)
              -> (right : SparseTreeList A l' acc')
              -> Am1 (tlist-amortized' A) A l
tListMergeAm\leq {l = l} {l' = l'} l\leql' left right with l <? l'
... | yes (s\leqs l\leql'-1) = tListMergeAm\leq l\leql'-1 left (empty:: right)
... | no  l\nltl' = tListMergeAm\equiv left (tlist-subst (sym $ \leq-antisym l\leql' (\nless=>\geq l\nltl')) right)

tListMergeAm :  {l l' acc acc' : bNat}
             -> (left : SparseTreeList A l acc)
             -> (right : SparseTreeList A l' acc')
             -> Am1 (tlist-amortized' A) A (l \glb l')
tListMergeAm {A = A} {l = l} {l' = l'} left right with \leq-total l l'
... | inj\_1 l\leql' = subst (Am1 (tlist-amortized' A) A) (sym $ m\leqn=>m\glbn\equivm l\leql') $ tListMergeAm\leq l\leql' left right
... | inj\_2 l'\leql = subst (Am1 (tlist-amortized' A) A) (sym $ m\leqn=>n\glbm\equivm l'\leql) $ tListMergeAm\leq l'\leql right left

tlist-merge-in-linear-time\equiv :  {{_ : Leq A}}
                               {l acc acc' : bNat}
                            -> (left : SparseTreeList A l acc)
                            -> (right : SparseTreeList A l acc')
                            -> atime-full1 (tListMergeAm\equiv left right) \bZ.\leq + (entries left + entries right)
tlist-merge-in-linear-time\equiv [] right = \bZ-Props.\leq-refl
tlist-merge-in-linear-time\equiv (empty:: left) [] = \bZ.+\leq+ (m\leqm+n (entries left) 0)
tlist-merge-in-linear-time\equiv ll@(empty:: left) rr@(empty:: right) = begin
        atime-full1 (tListMergeAm\equiv left right)
        \bZ.+ (0
             \ominus     am1-potential (tListMergeAm\equiv left right)
             \bZ.+ + am1-potential (tListMergeAm\equiv ll rr))

             \equiv\langle\rangle

        atime-full1 (tListMergeAm\equiv left right)
        \bZ.+ (0
             \ominus     am1-potential (tListMergeAm\equiv left right)
             \bZ.+ + am1-potential (tListMergeAm\equiv left right))

             \equiv\langle cong (\lambda x -> atime-full1 (tListMergeAm\equiv left right) \bZ.+ x) $
                0-a+[k+a]\equivk (am1-potential (tListMergeAm\equiv left right)) 0 \rangle

        atime-full1 (tListMergeAm\equiv left right) \bZ.+ + 0

            \equiv\langle \bZ-Props.+-identity\^r _ \rangle

        atime-full1 (tListMergeAm\equiv left right)

            \leq\langle tlist-merge-in-linear-time\equiv left right \rangle

        + (entries left + entries right) \qed
    where
        open \bZ-Props.\leq-Reasoning
tlist-merge-in-linear-time\equiv (empty:: left) (entry x :: right) = begin
        atime-full1 (tListMergeAm\equiv left right)
        \bZ.+ (0
            \ominus     am1-potential (tListMergeAm\equiv left right)
            \bZ.+ + (suc $ am1-potential $ tListMergeAm\equiv left right))

            \equiv\langle cong (\lambda x -> atime-full1 (tListMergeAm\equiv left right) \bZ.+ x) $ 0-a+suca\equiv1 (am1-potential $ tListMergeAm\equiv left right) \rangle

        atime-full1 (tListMergeAm\equiv left right) \bZ.+ + 1

            \leq\langle \bZ-Props.+-mono\^l-\leq (+ 1) (tlist-merge-in-linear-time\equiv left right) \rangle

        + (entries left + entries right) \bZ.+ + 1

            \equiv\langle cong (+_) $ +-comm _ 1 \rangle

        + suc (entries left + entries right)

            \equiv\langle cong (+_) $ sym $ +-suc _ _ \rangle

        + (entries left + suc (entries right))       \qed
    where
        open \bZ-Props.\leq-Reasoning
tlist-merge-in-linear-time\equiv (entry x :: left) [] = \bZ-Props.\leq-reflexive $ cong (\lambda x -> + suc x) $ sym $ +-identity\^r _
tlist-merge-in-linear-time\equiv (entry x :: left) (empty:: right) = begin
        atime-full1 (tListMergeAm\equiv left right)
        \bZ.+ (0
             \ominus     am1-potential (tListMergeAm\equiv left right)
             \bZ.+ + (suc $ am1-potential $ tListMergeAm\equiv left right))

            \equiv\langle cong (\lambda x -> atime-full1 (tListMergeAm\equiv left right) \bZ.+ x) $ 0-a+suca\equiv1 (am1-potential $ tListMergeAm\equiv left right) \rangle

        atime-full1 (tListMergeAm\equiv left right) \bZ.+ + 1

            \leq\langle \bZ-Props.+-mono\^l-\leq (+ 1) (tlist-merge-in-linear-time\equiv left right) \rangle

        + (entries left + entries right) \bZ.+ + 1

            \equiv\langle cong (+_) $ +-comm _ 1 \rangle

        + suc (entries left + entries right)

            \qed
    where
        open \bZ-Props.\leq-Reasoning
tlist-merge-in-linear-time\equiv ll@(entry x :: left) rr@(entry y :: right) = begin
        atime-full1 rec-merge
        \bZ.+ (suc (leadingEntries $ am1-eval rec-merge)
             \ominus     am1-potential rec-merge
             \bZ.+ + am1-potential nxt-merge)

            \equiv\langle cong (\lambda x -> atime-full1 rec-merge \bZ.+ x) $
               suca-b+c\equivsuc[a-b+c] (leadingEntries $ am1-eval rec-merge)
               (am1-potential rec-merge)
               (am1-potential nxt-merge) \rangle

        atime-full1 rec-merge
        \bZ.+ (+ 1 \bZ.+ (leadingEntries (am1-eval rec-merge)
             \ominus     am1-potential rec-merge
             \bZ.+ + am1-potential nxt-merge))

            \equiv\langle cong (\lambda x -> atime-full1 rec-merge \bZ.+ (+ 1 \bZ.+ x)) einsert \rangle

        atime-full1 rec-merge \bZ.+ (+ 2)

            \leq\langle \bZ-Props.+-mono\^l-\leq (+ 2) $ tlist-merge-in-linear-time\equiv left right \rangle

        + (entries left + entries right) \bZ.+ (+ 2)

            \equiv\langle \bZ-Props.+-comm (+ (entries left + entries right)) (+ 2) \rangle

        + 2 \bZ.+ + (entries left + entries right)

            \equiv\langle cong (+_) $ sym $ +-suc (suc $ entries left) (entries right) \rangle

        + suc (entries left + suc (entries right))

            \qed
    where
        open \bZ-Props.\leq-Reasoning
        open Relation.Binary.PropositionalEquality renaming (module \equiv-Reasoning to E)
        rec-merge = tListMergeAm\equiv left right
        nxt-merge = tListMergeAm\equiv ll rr
        einsert : leadingEntries (am1-eval rec-merge) \ominus am1-potential rec-merge \bZ.+ + am1-potential nxt-merge \equiv + 1
        einsert = E.begin
            leadingEntries (am1-eval rec-merge)
            \ominus     entries (am1-eval rec-merge)
            \bZ.+ + entries (am1-eval nxt-merge)

                E.\equiv\langle cong (\lambda x -> leadingEntries (am1-eval rec-merge)
                     \ominus     entries (am1-eval rec-merge)
                     \bZ.+ + entries x) $
                     apply-elim empty:: (insertTList\equiv (reduce $ link x y)
                     (am1-eval rec-merge)) \rangle

            leadingEntries (am1-eval rec-merge)
            \ominus entries (am1-eval rec-merge)
            \bZ.+ + entries (reduce $ insertTList\equiv (reduce $ link x y) (am1-eval rec-merge))

                E.\equiv\langle tlist-insert-pot-invariant (reduce $ link x y) (am1-eval rec-merge) \rangle

            + 1

                E.\qed

tlist-merge-in-linear-time\leq :  {{_ : Leq A}}
                               {l l' acc acc' : bNat}
                            -> (l\leql' : l \leq l')
                            -> (left : SparseTreeList A l acc)
                            -> (right : SparseTreeList A l' acc')
                            -> atime-full1 (tListMergeAm\leq l\leql' left right) \bZ.\leq + (entries left + entries right)
tlist-merge-in-linear-time\leq {l = l} {l' = l'} l\leql' left right with l <? l'
... | yes (s\leqs l\leql'-1) = tlist-merge-in-linear-time\leq l\leql'-1 left (empty:: right)
... | no l\nltl'  = begin
        atime-full1 (tListMergeAm\equiv left (tlist-subst (sym $ \leq-antisym l\leql' (\nlt=>\geq l\nltl')) right))

            \leq\langle tlist-merge-in-linear-time\equiv left (tlist-subst (sym $ \leq-antisym l\leql' (\nlt=>\geq l\nltl')) right) \rangle

        + (entries left + entries (tlist-subst (sym $ \leq-antisym l\leql' (\nlt=>\geq l\nltl')) right))

            \equiv\langle cong (\lambda x -> + (entries left + x)) $ sym $ tlist-subst-elim entries (sym $ \leq-antisym l\leql' (\nlt=>\geq l\nltl')) right \rangle

        + (entries left + entries right) \qed
    where
        open \bZ-Props.\leq-Reasoning

tlist-merge-in-linear-time :  {{_ : Leq A}}
                              {l l' acc acc' : bNat}
                           -> (left : SparseTreeList A l acc)
                           -> (right : SparseTreeList A l' acc')
                           -> atime-full1 (tListMergeAm left right) \bZ.\leq + (entries left + entries right)
tlist-merge-in-linear-time {A = A} {l = l} {l' = l'} left right with \leq-total l l'
... | inj\_1 l\leql' = begin
        atime-full1 (subst (Am1 (tlist-amortized' A) A) (sym $ m\leqn=>m\glbn\equivm l\leql') $ tListMergeAm\leq l\leql' left right)

            \equiv\langle subst-appl' atime-full1 (sym $ m\leqn=>m\glbn\equivm l\leql') $ tListMergeAm\leq l\leql' left right \rangle

        atime-full1 (tListMergeAm\leq l\leql' left right)

            \leq\langle tlist-merge-in-linear-time\leq l\leql' left right \rangle

        + (entries left + entries right) \qed
    where
        open \bZ-Props.\leq-Reasoning
... | inj\_2 l'\leql = begin
        atime-full1 (subst (Am1 (tlist-amortized' A) A) (sym $ m\leqn=>n\glbm\equivm l'\leql) $ tListMergeAm\leq l'\leql right left)

            \equiv\langle subst-appl' atime-full1 (sym $ m\leqn=>n\glbm\equivm l'\leql) $ tListMergeAm\leq l'\leql right left \rangle

        atime-full1 (tListMergeAm\leq l'\leql right left)

            \leq\langle tlist-merge-in-linear-time\leq l'\leql right left \rangle

        + (entries right + entries left)

            \equiv\langle cong (+_) $ +-comm (entries right) (entries left) \rangle

        + (entries left + entries right) \qed
    where
        open \bZ-Props.\leq-Reasoning

merge-in-log-time :  {{_ : Leq A}}
                     {l l' acc acc' : bNat}
                  -> (left : SparseTreeList A l acc)
                  -> (right : SparseTreeList A l' acc')
                  -> atime-full1 (tListMergeAm left right) \bZ.\leq + 2 * 1+\lfloorlog\_2 acc \lub acc' \rfloor
merge-in-log-time {acc = acc} {acc' = acc'} left right = \bZ\leq.begin
        atime-full1 (tListMergeAm left right)

            \bZ\leq.\leq\langle tlist-merge-in-linear-time left right \rangle

        + (entries left + entries right)

            \bZ\leq.\leq\langle \bZ.+\leq+ $ begin

                entries left + entries right                     \leq\langle +-mono\^l-\leq _ $ len\leq\lfloorlog\_2acc\rfloor left \rangle

                1+\lfloorlog\_2 acc \rfloor + entries right                    \leq\langle +-mono\^l-\leq _ $ 1+\lfloorlog\_2\rfloor-mono $ m\leqm\lubn acc acc' \rangle

                1+\lfloorlog\_2 acc \lub acc' \rfloor + entries right             \leq\langle +-mono\^r-\leq _ $ len\leq\lfloorlog\_2acc\rfloor right \rangle

                1+\lfloorlog\_2 acc \lub acc' \rfloor + 1+\lfloorlog\_2 acc' \rfloor            \leq\langle +-mono\^r-\leq _ $ 1+\lfloorlog\_2\rfloor-mono $ n\leqm\lubn acc acc' \rangle


                1+\lfloorlog\_2 acc \lub acc' \rfloor + 1+\lfloorlog\_2 acc \lub acc' \rfloor      \equiv\langle\rangle


                2 * 1+\lfloorlog\_2 acc \lub acc' \rfloor                         \qed

            \rangle

        + (2 * 1+\lfloorlog\_2 acc \lub acc' \rfloor)

            \bZ\leq.\qed
    where
        open \bZ-Props renaming (module \leq-Reasoning to \bZ\leq) using ()
        open \leq-Reasoning
\end{lstlisting}
\begin{lstlisting}[caption={Finding the minimum element},label={lst:appendix:heap:min}]
findMin : {l acc : bNat} -> SparseTreeList A l (suc acc) -> DecTree A A 1+\lfloorlog\_2 (suc acc) \rfloor
findMin ts = delay-\leq (len\leq\lfloorlog\_2acc\rfloor ts) $ findMin' ts
    where
        findMin'' : {l acc : bNat} -> A -> (ts : SparseTreeList A l acc) -> DecTree A A (entries ts)
        findMin'' a [] = return a
        findMin'' a (empty:: ts) = findMin'' a ts
        findMin'' a (entry node :: ts) = if' a \leq? (tVal node) then findMin'' a ts else findMin'' (tVal node) ts

        findMin' : {l acc : bNat} -> (ts : SparseTreeList A l (suc acc)) -> DecTree A A (entries ts)
        findMin' (empty:: ts) = findMin' ts
        findMin' (entry node :: ts) = delay' 1 $ findMin'' (tVal node) ts
\end{lstlisting}
\begin{lstlisting}[caption={Removing the minimum element},label={lst:appendix:heap:remove}]
cum-acc : {l : bNat} -> DescList (BinomialTree A) l -> bNat
cum-acc D[ _ ] = 1
cum-acc (_D::_ {l = l} _ dl) = cum-acc dl + 2 ^ (suc l)

cum-acc\equiv2^l : {l : bNat} -> (dl : DescList (BinomialTree A) l) -> suc (cum-acc dl) \equiv 2 ^ (suc l)
cum-acc\equiv2^l D[ _ ] = refl
cum-acc\equiv2^l {l = l} (_D::_ {l = l-1} _ dl) = cong (_+ 2 ^ l) $ cum-acc\equiv2^l dl

inner-acc : {l : bNat} -> BinomialTree A l -> bNat
inner-acc (Leaf _) = 0
inner-acc (Node _ ts) = cum-acc ts

inner-acc\equiv2^l : {l : bNat} -> (t : BinomialTree A l) -> suc (inner-acc t) \equiv 2 ^ l
inner-acc\equiv2^l (Leaf _) = refl
inner-acc\equiv2^l (Node _ ts) = cum-acc\equiv2^l ts

desclist-2-sparselist : {l : bNat} -> (dl : DescList (BinomialTree A) l) -> SparseTreeList A 0 (cum-acc dl)
desclist-2-sparselist dl = tlist-subst-acc (+-identity\^r $ cum-acc dl) $ dl-2-sparse dl []
    where
        dl-2-sparse : {l acc : bNat} -> (dl : DescList (BinomialTree A) l) -> SparseTreeList A (suc l) acc -> SparseTreeList A 0 (cum-acc dl + acc)
        dl-2-sparse {acc = acc} D[ x ] ts = entry_::_ {acc'\equiv2^l+acc = refl} x ts
        dl-2-sparse {l = l} {acc = acc} (x D:: dl) ts = tlist-subst-acc (sym $ +-assoc (cum-acc dl) (2 ^ l) acc) $ dl-2-sparse dl (entry_::_ {acc'\equiv2^l+acc = refl} x ts)


inner-trees : {l : bNat} -> (t : BinomialTree A l) -> SparseTreeList A 0 (inner-acc t)
inner-trees (Leaf _) = []
inner-trees (Node _ ts) = desclist-2-sparselist ts

record RemoveTree (A : Set a) (l : bNat) (acc : bNat) : Set a where
    field
        {l'} : bNat
        {acc'} : bNat
        min : A
        tree : BinomialTree A l'
        rem-heap : SparseTreeList A l acc'
        full-heap : SparseTreeList A l acc
        acc\equivacc'+inner : acc \equiv acc' + suc (inner-acc tree)


find-and-remove-min-tree : {l acc : bNat} -> (ts : SparseTreeList A l (suc acc)) -> DecTree A (RemoveTree A l (suc acc)) 1+\lfloorlog\_2 suc acc \rfloor
find-and-remove-min-tree ts = delay-\leq (len\leq\lfloorlog\_2acc\rfloor ts) $ find-and-remove-min' ts
    where
        ext-rt-empty : {l acc : bNat} -> RemoveTree A (suc l) acc -> RemoveTree A l acc
        ext-rt-empty record { min = min ; tree = tree ; rem-heap = rem-heap ; full-heap = full-heap ; acc\equivacc'+inner = accinn}
                     = record { min = min ; tree = tree ; rem-heap = empty:: rem-heap ; full-heap = empty:: full-heap ; acc\equivacc'+inner = accinn}
        ext-rt-entry : {l acc : bNat} -> BinomialTree A l -> RemoveTree A (suc l) acc -> RemoveTree A l (2 ^ l + acc)
        ext-rt-entry {l = l} t record { min = min ; tree = tree ; rem-heap = rem-heap ; full-heap = full-heap ; acc\equivacc'+inner = accinn }
                     = record {
                          min = min
                       ; tree = tree
                       ; rem-heap =  entry_::_ {acc'\equiv2^l+acc = refl} t rem-heap
                       ; full-heap = entry_::_ {acc'\equiv2^l+acc = refl} t full-heap
                       ; acc\equivacc'+inner = trans (cong (\lambda x -> 2 ^ l + x) accinn) (sym $ +-assoc (2 ^ l) _ _)
                       }
        swap-rt : {l acc : bNat} -> BinomialTree A l -> RemoveTree A (suc l) acc -> RemoveTree A l (2 ^ l + acc)
        swap-rt {acc = acc} node record { full-heap = full-heap ; acc\equivacc'+inner = acc+inn }
                = record {
                    min = (tVal node)
                  ; tree = node
                  ; rem-heap = empty:: full-heap
                  ; full-heap = entry_::_ {acc'\equiv2^l+acc = refl} node full-heap
                  ; acc\equivacc'+inner = trans (cong (_+ acc) $ sym $ inner-acc\equiv2^l node) (+-comm _ acc)
                  }
        find-and-remove-min' : {l acc : bNat} -> (ts : SparseTreeList A l (suc acc)) -> DecTree A (RemoveTree A l (suc acc)) (entries ts)
        find-and-remove-min' (empty:: ts) = find-and-remove-min' ts <&> \lambda rt -> ext-rt-empty rt
        find-and-remove-min' (entry_::_ {acc = acc@(suc acc-1)} {acc'\equiv2^l+acc = pf} node ts) =
            height-\equiv (+-comm _ 1) $ do
                rt <- find-and-remove-min' ts
                if' (RemoveTree.min rt) \leq? (tVal node)
                then return (subst (RemoveTree _ _) (sym pf) $ ext-rt-entry node rt)
                else return (subst (RemoveTree _ _) (sym pf) $ swap-rt node rt)
        find-and-remove-min' {l = l} (entry_::_ {acc = zero} {acc'\equiv2^l+acc = pf} node ts) =
                delay-\leq z\leqn $
                return $ subst (RemoveTree _ _) (sym pf) $
                    record { min = (tVal node)
                           ; tree = node
                           ; rem-heap = []
                           ; full-heap = entry_::_ {acc'\equiv2^l+acc = refl} node []
                           ; acc\equivacc'+inner = trans (+-identity\^r $ 2 ^ l) (sym $ inner-acc\equiv2^l node)
                           }

deleteMin : {l acc : bNat} -> (ts : SparseTreeList A l (suc acc)) -> Am1 (tlist-amortized' A) A 0
deleteMin {A = A} {l = l} ts =
        Am1.init-comp {am = tlist-amortized' A}
            rem
            \lambda rt -> tListMergeAm\leq z\leqn (inner-trees $ RemoveTree.tree rt) (RemoveTree.rem-heap rt)
    where
        rem = find-and-remove-min-tree ts


deleteMin-in-log-time :  {{_ : Leq A}}
                         {l acc : bNat}
                      -> (ts : SparseTreeList A l (suc acc))
                      -> atime-full1 (deleteMin ts) \bZ.\leq + 3 * 1+\lfloorlog\_2 suc acc \rfloor
deleteMin-in-log-time {acc = acc} ts = \bZ-Props.+-mono\^r-\leq (+ 1+\lfloorlog\_2 suc acc \rfloor) $ begin
        atime-full1 (tListMergeAm\leq z\leqn (inner-trees $ RemoveTree.tree rem') (RemoveTree.rem-heap rem'))
            \leq\langle tlist-merge-in-linear-time\leq z\leqn (inner-trees $ RemoveTree.tree rem') (RemoveTree.rem-heap rem') \rangle
        + (entries (inner-trees $ RemoveTree.tree rem') + entries (RemoveTree.rem-heap rem'))
            \leq\langle \bZ-Props.+-mono\^r-\leq (+ (entries $ inner-trees $ RemoveTree.tree rem')) $ \bZ.+\leq+ $ len\leq\lfloorlog\_2acc\rfloor (RemoveTree.rem-heap rem') \rangle
        + (entries (inner-trees $ RemoveTree.tree rem') + 1+\lfloorlog\_2 RemoveTree.acc' rem' \rfloor)
            \leq\langle \bZ-Props.+-mono\^r-\leq (+ entries (inner-trees $ RemoveTree.tree rem')) $ \bZ.+\leq+ $ 1+\lfloorlog\_2\rfloor-mono acc'\leqacc \rangle
        + (entries (inner-trees $ RemoveTree.tree rem') + 1+\lfloorlog\_2 suc acc \rfloor)
            \leq\langle \bZ-Props.+-mono\^l-\leq (+ 1+\lfloorlog\_2 suc acc \rfloor) $ \bZ.+\leq+ $ len\leq\lfloorlog\_2acc\rfloor $ inner-trees $ RemoveTree.tree rem' \rangle
        + (1+\lfloorlog\_2 inner-acc $ RemoveTree.tree rem' \rfloor + 1+\lfloorlog\_2 suc acc \rfloor)
            \leq\langle \bZ-Props.+-mono\^l-\leq (+ 1+\lfloorlog\_2 suc acc \rfloor) $ \bZ.+\leq+ $ 1+\lfloorlog\_2\rfloor-mono $ n\leq1+n _ \rangle
        + (1+\lfloorlog\_2 suc $ inner-acc $ RemoveTree.tree rem' \rfloor + 1+\lfloorlog\_2 suc acc \rfloor)
            \leq\langle \bZ-Props.+-mono\^l-\leq (+ 1+\lfloorlog\_2 suc acc \rfloor) $ \bZ.+\leq+ $ 1+\lfloorlog\_2\rfloor-mono accinner\leqacc \rangle
        + 2 * 1+\lfloorlog\_2 suc acc \rfloor \qed
    where
        open \bZ-Props.\leq-Reasoning
        rem = find-and-remove-min-tree ts
        rem' = reduce rem
        acc'\leqacc = m+n\leqo=>m\leqo (RemoveTree.acc' rem') (\leq-reflexive $ sym $ RemoveTree.acc\equivacc'+inner rem')
        accinner\leqacc = m+n\leqo=>n\leqo (RemoveTree.acc' rem') (\leq-reflexive $ sym $ RemoveTree.acc\equivacc'+inner rem')
\end{lstlisting}